```haskell
add :: Nat -> Nat -> Nat
add Zero m = m
add (Succ n) m = Succ (add n m)
```

Proving:

```haskell
add n m = add m n
```

By properties:

Identity:

```haskell
add n Zero = n
```

Linearity in Second Argument:

```haskell
add n (Succ m) = Succ (add n m)
```

Base Case:

```haskell
add Zero m
-- applying add
= m
-- unapplying identity property
= add m Zero
```

Inductive Case:

```haskell
add (Succ k) m
-- applying add
= Succ (add k m)
-- inductive hypothesis
= Succ (add m k)
-- applying linearity property
= add m (Succ k)
```
